Rename POS_INT32_LIMIT to INT32_MAX_LIMIT

src/StandardLibrary/UInt.dfy
@@ -10,7 +10,7 @@ module {:extern "STLUInt"} StandardLibrary.UInt {
 
   const UINT16_LIMIT := 0x1_0000
   const UINT32_LIMIT := 0x1_0000_0000
-  const POS_INT32_LIMIT := 0x8000_0000
+  const INT32_MAX_LIMIT := 0x8000_0000
 
   predicate method UInt8Less(a: uint8, b: uint8) { a < b }
 
